chore: redesign API about `isEmpty` and `size`

Algorithm/Data/Classes/ToMultiset.lean
@@ -4,10 +4,20 @@ Released under Apache 2.0 license as described in the file LICENSE.
 Authors: Yuyang Zhao
 -/
 import Algorithm.Data.Classes.Erase
-import Algorithm.Data.Classes.Size
 import Mathlib.Data.Multiset.AddSub
 
 variable {C α : Type*}
+
+class Membership.IsEmpty (C : Type*) {α : outParam Type*} [Membership α C] where
+  isEmpty : C → Bool
+  isEmpty_iff_forall_not_mem {c} : isEmpty c ↔ ∀ a, a ∉ c
+export Membership.IsEmpty (isEmpty isEmpty_iff_forall_not_mem)
+
+lemma isEmpty_eq_false_iff_exists_mem [Membership α C] [Membership.IsEmpty C] {c : C} :
+    isEmpty c = false ↔ ∃ a, a ∈ c := by
+  rw [← Bool.eq_false_eq_not_eq_true, not_iff_comm, isEmpty_iff_forall_not_mem]
+  push_neg
+  rfl
 
 @[mk_iff]
 class LawfulEmptyCollection (C : Type*) (α : outParam Type*)
@@ -15,14 +25,33 @@ class LawfulEmptyCollection (C : Type*) (α : outParam Type*)
   not_mem_empty (x : α) : x ∉ (∅ : C)
 export LawfulEmptyCollection (not_mem_empty)
 
-class ToMultiset (C : Type*) (α : outParam Type*) extends Membership α C, Size C where
+class ToMultiset (C : Type*) (α : outParam Type*) extends Membership α C, Membership.IsEmpty C where
   toMultiset : C → Multiset α
   mem c a := a ∈ toMultiset c
   mem_toMultiset {x c} : x ∈ toMultiset c ↔ x ∈ c := by rfl
-  size_eq_card_toMultiset c : size c = Multiset.card (toMultiset c)
-export ToMultiset (toMultiset mem_toMultiset size_eq_card_toMultiset)
+export ToMultiset (toMultiset mem_toMultiset)
 
 attribute [simp] mem_toMultiset
+
+/--
+The size function derived from `ToMultiset`.
+
+Use `size` for computation whenever possible, as it is usually faster.
+-/
+def sizeTM [ToMultiset C α] (c : C) : Nat :=
+  (toMultiset c).card
+
+lemma card_toMultiset [ToMultiset C α] (c : C) : (toMultiset c).card = sizeTM c := rfl
+
+lemma sizeTM_eq_card_toMultiset [ToMultiset C α] (c : C) : sizeTM c = (toMultiset c).card :=
+  rfl
+
+class Size (C : Type*) {α : outParam Type*} [ToMultiset C α] where
+  size : C → Nat
+  size_eq_sizeTM c : size c = sizeTM c
+export Size (size size_eq_sizeTM)
+
+attribute [simp] size_eq_sizeTM
 
 class ToMultiset.LawfulInsert (C : Type*) (α : outParam Type*)
     [ToMultiset C α] [Insert α C] : Prop where
@@ -39,17 +68,35 @@ export LawfulErase (toMultiset_erase)
 
 attribute [simp] toMultiset_erase
 
-section ToMultiset
+section instances
+
+instance : Membership.IsEmpty (List α) where
+  isEmpty := List.isEmpty
+  isEmpty_iff_forall_not_mem := by simp [List.eq_nil_iff_forall_not_mem]
 
 instance : ToMultiset (List α) α where
   toMultiset := (↑)
   mem_toMultiset := .rfl
-  size_eq_card_toMultiset _ := rfl
+
+instance : Size (List α) where
+  size := List.length
+  size_eq_sizeTM _ := rfl
+
+instance : Membership.IsEmpty (Array α) where
+  isEmpty := Array.isEmpty
+  isEmpty_iff_forall_not_mem := by simp [Array.eq_empty_iff_forall_not_mem]
 
 instance : ToMultiset (Array α) α where
   toMultiset c := ↑c.toList
   mem_toMultiset := Array.mem_def.symm
-  size_eq_card_toMultiset _ := by simp [size]
+
+instance : Size (Array α) where
+  size := Array.size
+  size_eq_sizeTM _ := rfl
+
+end instances
+
+section ToMultiset
 
 variable [ToMultiset C α]
 
@@ -70,14 +117,34 @@ lemma toMultiset_empty [LawfulEmptyCollection C α] :
 end LawfulEmptyCollection
 
 @[simp]
-lemma toMultiset_of_isEmpty {c : C} (h : isEmpty c) : toMultiset c = 0 := by
-  simpa [size_eq_card_toMultiset] using h
-
-@[simp]
 lemma toMultiset_list (l : List α) : toMultiset l = ↑l := rfl
 
+section IsEmpty
+
+lemma isEmpty_iff_sizeTM_eq_zero {c : C} : isEmpty c ↔ sizeTM c = 0 := by
+  simp [isEmpty_iff_forall_not_mem, sizeTM, Multiset.eq_zero_iff_forall_notMem]
+
+lemma isEmpty_iff_size_eq_zero [Size C] {c : C} : isEmpty c ↔ size c = 0 := by
+  simp [isEmpty_iff_sizeTM_eq_zero]
+
+lemma isEmpty_eq_decide_sizeTM (c : C) : isEmpty c = decide (sizeTM c = 0) := by
+  simp only [← isEmpty_iff_sizeTM_eq_zero, Bool.decide_coe]
+
+lemma isEmpty_eq_sizeTM_beq_zero (c : C) : isEmpty c = (sizeTM c == 0) := by
+  rw [isEmpty_eq_decide_sizeTM]
+  cases sizeTM c <;> rfl
+
+lemma toMultiset_iff_isEmpty {c : C} : isEmpty c ↔ toMultiset c = 0 := by
+  simp only [isEmpty_iff_sizeTM_eq_zero, sizeTM, Multiset.card_eq_zero]
+
+alias ⟨toMultiset_of_isEmpty, _⟩ := toMultiset_iff_isEmpty
+
+attribute [simp] toMultiset_of_isEmpty
+
 lemma ToMultiset.not_isEmpty_of_mem {c : C} {x} (hx : x ∈ c) : ¬isEmpty c := by
-  simpa [size_eq_card_toMultiset, Multiset.eq_zero_iff_forall_notMem] using ⟨x, hx⟩
+  simpa [sizeTM, isEmpty_iff_sizeTM_eq_zero, Multiset.eq_zero_iff_forall_notMem] using ⟨x, hx⟩
+
+end IsEmpty
 
 variable [DecidableEq α]
 
